some more tweaks to avoid destructing character_string_t

dice/src/l0/L0.X509.AliasKeyTBS.Subject.fst
@@ -9,6 +9,10 @@ module B32 = FStar.Bytes
 
 #set-options "--z3rlimit 512 --fuel 0 --ifuel 0 --using_facts_from '* -FStar.Tactics -FStar.Reflection'"
 
+#set-options "--__temp_no_proj L0.X509.AliasKeyTBS.Subject"
+
+let decl = ()
+
 let aliasKeyTBS_subject_payload_t' = (
   x509_RDN_x520_attribute_t COMMON_NAME  IA5_STRING `tuple2`
   x509_RDN_x520_attribute_t ORGANIZATION IA5_STRING `tuple2`
