dice/src/l0/L0.X509.AliasKeyTBS.Subject.fsti
@@ -11,6 +11,10 @@ module B32 = FStar.Bytes
 
 #set-options "--z3rlimit 128 --fuel 0 --ifuel 0 --using_facts_from '* -FStar.Tactics -FStar.Reflection'"
 
+#set-options "--__temp_no_proj L0.X509.AliasKeyTBS.Subject"
+
+val decl : unit
+
 noeq
 type aliasKeyTBS_subject_payload_t = {
   aliasKeyTBS_subject_Common      : x509_RDN_x520_attribute_t COMMON_NAME  IA5_STRING;
